sepcomp-reserved/extension.v
@@ -33,34 +33,39 @@ Module Extension. Section Extension. Variables
 
  Record Sig := Make {
   proj_max_cores: xT -> nat;
-  proj_core: forall i:nat, xT -> option (cT i); 
-  proj_core_max: forall i s, i>=proj_max_cores s -> proj_core i s=None;
+  proj_core: forall (i j:nat), xT -> option (cT j); (*i is thread_id; j is module type index*)
+  proj_core_max: forall i j s, i>=proj_max_cores s -> proj_core i j s=None;
   active : xT -> nat; 
-  active_proj_core : forall s, exists c, proj_core (active s) s=Some c;
+  active_proj_core : forall s, exists j c, proj_core (active s) j s=Some c;
   proj_zint: xT -> Zint; 
   proj_zext: Z -> Zext;
   zmult: Zint -> Zext -> Z;
   zmult_proj: forall zint zext, proj_zext (zmult zint zext)=zext;
+
+  proj_core_types: forall (i u u': nat) c c' s,
+    proj_core i u s = Some c -> 
+    proj_core i u' s = Some c' -> 
+    u=u';
  
   zint_invar_after_external: forall ef sig args ret s s',
    at_external esem s = Some (ef, sig, args) -> 
    after_external esem ret s = Some s' -> proj_zint s=proj_zint s';
 
   handled (ef: AST.external_function) :=
-   forall (s: xT) (c: cT (active s)) sig args,
-    proj_core (active s) s = Some c ->
-    at_external (csem (active s)) c = Some (ef, sig, args) ->
+   forall (s: xT) j (c: cT j) sig args,
+    proj_core (active s) j s = Some c ->
+    at_external (csem j) c = Some (ef, sig, args) ->
     at_external esem s = None;
 
   linkable: linkable proj_zext handled csig esig;
 
   handled_invar: 
-   forall s c s' c' ef sig args sig' args',
-    proj_core (active s) s = Some c ->
-    at_external (csem (active s)) c = Some (ef, sig, args) ->
+   forall j s c s' c' ef sig args sig' args',
+    proj_core (active s) j s = Some c ->
+    at_external (csem j) c = Some (ef, sig, args) ->
     at_external esem s = None -> 
-    proj_core (active s') s' = Some c' ->
-    at_external (csem (active s')) c' = Some (ef, sig', args') ->
+    proj_core (active s') j s' = Some c' ->
+    at_external (csem j) c' = Some (ef, sig', args') ->
     at_external esem s' = None
  }.
 
@@ -89,20 +94,20 @@ Section CoreCompatible. Variables
  (csem: forall i:nat, CoreSemantics (gT i) (cT i) M (dT i)) (** a set of core semantics *)
  (csig: ef_ext_spec M Z). (** client signature *)
 
- Variables (ge: G) (genv_map : forall i:nat, gT i).
- Variable E: Extension.Sig Z Zint Zext esem esig gT dT cT csem csig.
-
  Import Extension.
+
+ Variables (ge: G) (genv_map : forall u: nat, gT u).
+ Variable E: Extension.Sig Z Zint Zext esem esig gT dT cT csem csig.
 
  Inductive core_compatible: Type := CoreCompatible: forall
  (** When the active thread is runnable, a step in the extended semantics can be
     tracked back to a corestep of the active thread. *)
- (runnable_corestep: forall s m s' m' c,
-   runnable (csem (active E s)) c=true -> 
-   proj_core E (active E s) s = Some c -> 
+ (runnable_corestep: forall j s m s' m' c,
+   runnable (csem j) c=true -> 
+   proj_core E (active E s) j s = Some c -> 
    corestep esem ge s m s' m' -> 
-   exists c', corestep (csem (active E s)) (genv_map (active E s)) c m c' m' /\ 
-    proj_core E (active E s) s' = Some c') 
+   exists c', corestep (csem j) (genv_map j) c m c' m' /\ 
+    proj_core E (active E s) j s' = Some c') 
 
  (** After a corestep of the active inner core, the active thread's new
     corestate is appropriately injected into the extended state. Note that 
@@ -112,62 +117,61 @@ Section CoreCompatible. Variables
     a relation, or equivalently, have proj_core project a /set/ of corestates; 
     but at the current stage, the conveniences of proj_core-as-function appear to 
     outweigh the disadvantages. *)
- (corestep_pres: forall s (c: cT (active E s)) m c' s' m1' m2',
-   proj_core E (active E s) s = Some c -> 
-   corestep (csem (active E s)) (genv_map (active E s)) c m c' m1' -> 
+ (corestep_pres: forall j s (c: cT j) m c' s' m1' m2',
+   proj_core E (active E s) j s = Some c -> 
+   corestep (csem j) (genv_map j) c m c' m1' -> 
    corestep esem ge s m s' m2' -> 
    active E s = active E s' /\ 
-   proj_core E (active E s) s' = Some c' /\
+   proj_core E (active E s) j s' = Some c' /\
    m1'=m2')
 
  (** A corestep of the currently active core forces a corestep of the 
     extended semantics *)
- (corestep_prog: forall s (c: cT (active E s)) m c' m',
-   proj_core E (active E s) s = Some c -> 
-   corestep (csem (active E s)) (genv_map (active E s)) c m c' m' -> 
+ (corestep_prog: forall j s (c: cT j) m c' m',
+   proj_core E (active E s) j s = Some c -> 
+   corestep (csem j) (genv_map j) c m c' m' -> 
    exists s', corestep esem ge s m s' m')
 
  (** Other cores remain unchanged after coresteps of the active core. *)
- (corestep_others_forward: forall s s' (c: cT (active E s')) m c' m',
+ (corestep_others_forward: forall j s s' (c: cT j) m c' m',
    active E s=active E s' -> 
-   proj_core E (active E s') s' = Some c' -> 
-   corestep (csem (active E s')) (genv_map (active E s')) c m c' m' -> 
+   proj_core E (active E s') j s' = Some c' -> 
+   corestep (csem j) (genv_map j) c m c' m' -> 
    corestep esem ge s m s' m' -> 
-   forall j, (active E s)<>j -> proj_core E j s = proj_core E j s')
- (corestep_others_backward: forall s c m s' c' m' n,
-   proj_core E (active E s) s = Some c -> 
-   corestepN (csem (active E s)) (genv_map (active E s)) n c m c' m' -> 
+   forall i u, (active E s)<>i -> proj_core E i u s = proj_core E i u s')
+ (corestep_others_backward: forall j s c m s' c' m' n,
+   proj_core E (active E s) j s = Some c -> 
+   corestepN (csem j) (genv_map j) n c m c' m' -> 
    corestepN esem ge n s m s' m' -> 
-   forall j, (active E s)<>j -> proj_core E j s = proj_core E j s')
+   forall i u, (active E s)<>i -> proj_core E i u s = proj_core E i u s')
 
  (** The active core id doesn't change along active coresteps. *)
- (after_ext_pres: forall s (c: cT (active E s)) c' s' retv,
-   proj_core E (active E s) s = Some c -> 
-   after_external (csem (active E s)) retv c = Some c' -> 
+ (after_ext_pres: forall j s (c: cT j) c' s' retv,
+   proj_core E (active E s) j s = Some c -> 
+   after_external (csem j) retv c = Some c' -> 
    after_external esem retv s = Some s' -> 
    active E s=active E s')
 
  (** Extension states can be updated to match after_external on the 
     active core. *)
- (after_ext_prog: forall s (c: cT (active E s)) c' retv,
-   proj_core E (active E s) s = Some c -> 
-   after_external (csem (active E s)) retv c = Some c' -> 
+ (after_ext_prog: forall j s (c: cT j) c' retv,
+   proj_core E (active E s) j s = Some c -> 
+   after_external (csem j) retv c = Some c' -> 
    exists s', after_external esem retv s = Some s' /\
-    proj_core E (active E s) s' = Some c')
+    proj_core E (active E s) j s' = Some c')
 
  (** after_external on extension cores leaves all but the active corestate
     unchanged. *)
- (after_ext_others: forall s s' retv,
+ (after_ext_others: forall j0 s s' retv,
    after_external esem retv s = Some s' -> 
    forall j, (active E s)<>j -> 
-    proj_core E j s = proj_core E j s')
+    proj_core E j j0 s = proj_core E j j0 s')
 
  (*Hypothesis repeated from extension signature to get around a bug in [Program]*)
  (at_extern_call: forall s ef sig args,
    at_external esem s = Some (ef, sig, args) -> 
-   exists c, proj_core E (active E s) s = Some c /\
-    at_external (csem (active E s)) c = Some (ef, sig, args)),
+   exists j c, proj_core E (active E s) j s = Some c /\
+    at_external (csem j) c = Some (ef, sig, args)),
  core_compatible.
 
 End CoreCompatible.
-
